Update

4.1/41_exercise_sheet.lean
@@ -16,7 +16,13 @@ lemma exists_minimal_arg.aux (f : ℕ → ℕ) :
   begin
     -- this works thanks to `classical.prop_decidable`
     by_cases (∃n', f n' < x),
-    repeat { sorry }
+    cases h,
+    apply exists_minimal_arg.aux _ h_w _,
+    apply x,
+    apply le_e
+    cases eq,
+    
+    
   end
 
 /- Now this interesting lemma falls off: -/
@@ -44,7 +50,65 @@ namespace exercise
 
 instance int.rel : setoid (ℕ × ℕ) :=
 { r     := λa b, a.1 + b.2 = b.1 + a.2,
-  iseqv := sorry }
+  iseqv :=
+  ⟨ (assume a, rfl),
+    (assume a b eq, eq.symm),
+    (assume a b c fst snd, 
+    have (a.fst + c.snd) + b.snd = (c.fst + a.snd) + b.snd := 
+    calc (a.fst + c.snd) + b.snd = (a.fst + b.snd) + c.snd    : by ac_refl
+                             ... =  a.snd + (b.fst + c.snd)   : by {rw[fst], ac_refl}
+                             ... =  (c.fst + a.snd ) + b.snd  : by {rw[snd], ac_refl},
+    calc (a.fst + c.snd) = (c.fst + a.snd)                    : by {apply eq_of_add_eq_add_right this})⟩ 
+    }
+
+
+def count {α: Type} (a: α) [decidable_eq α]: list α → ℕ
+| [] := 0
+| (x :: xs) := if x = a then 1 + count xs else count xs
+
+#reduce count 2[2,2,2,2]
+
+
+  instance list.rel (α: Type) : setoid (list α) :=
+{ r     := λxs ys, ∀x, count x xs = count x ys,
+  iseqv := 
+  ⟨ (assume xs, begin simp end),
+  (assume xs ys a b c, begin simp *, end)
+  (assume xs ys zs xs_zs ys_zs, by simp *) ⟩ }
+
+lemma rel_set {α: Type} (xs ys: list α): xs ≈ ys ↔ count xs = count ys := sorry
+
+
+def multiset (α: Type): Type := quotient (list.rel α)
+
+-- lemma counter {α: Type} (xs xs_ys ys ys_xs: list α): count (xs ++ ys) = count xs + count ys
+
+lemma r_reflexive {α: Type} (xs : list α) : r count xs xs 
+lemma r_symmetric (xs ys : list α) : r xs ys → r ys xs 
+lemma r_transitive (xs ys zs : listα) : r xs ys→r ys zs→r xs zs
+
+def empty_mset {α: Type}: multiset α :=  ⟦[]⟧ 
+def singleton_mset {α: Type} (a: α) : multiset α :=  ⟦[a]⟧
+def sum_mset {α: Type} (A: multiset α) (B: multiset α) : multiset α :=
+quotient.lift_on₂ A B (λxs ys, ⟦xs ++ ys⟧ )
+begin 
+intros xs ys xs_ys ys_xs,
+intro xs1,
+intro ys1,
+apply quotient.sound,
+simp[rel_set],
+simp[rel_set] at xs1,
+simp[rel_set] at ys1,
+
+end
+
+
+inductive finite {α: Type}: set α → Prop
+|empty : finite ∅
+|singleton (a: α) : finite({a})
+|union (A B: set α) (h: finite A) (s: finite B) : finite(A ∪ B)
+
+def multiset2 (α: Type) : Type := subtype (finite α)
 
 @[simp] lemma rel_iff (a b : ℕ × ℕ) : a ≈ b ↔ a.1 + b.2 = b.1 + a.2 := iff.rfl
 
@@ -53,14 +117,31 @@ def int : Type := quotient int.rel
 /- 2.1. Define negation using `quotient.lift_on`. -/
 
 def neg (a : int) : int :=
-sorry
+quotient.lift_on a (λpn, ⟦(pn.2, pn.1)⟧ )
+begin
+intros pn b pnb,
+simp[rel_iff],
+apply quotient.sound,
+simp,
+simp at pnb,
+rw[pnb]
+end
 
 /- 2.2. Prove the following lemmas. -/
 
-lemma neg_mk (p n : ℕ) : neg ⟦(p, n)⟧ = ⟦(n, p)⟧ :=
-sorry
+lemma neg_mk (p n : ℕ) : neg ⟦(p, n)⟧ = ⟦(n, p)⟧:=
+begin
+unfold neg,
+apply quotient.sound,
+rw[rel_iff]
+end
 
 lemma neg_neg (a : int) : neg (neg a) = a :=
-sorry
+begin
+apply quotient.induction_on a,
+intro n,
+cases n,
+refl
+end
 
 end exercise
